\documentclass{bmstu}

\begin{document}

\section*{Метод скользящего окна}

\begin{equation}
    H(X) = -\sum_{i = 0}^{255} (p_{i} \cdot \log_{2}p_{i}).
\end{equation}

\begin{equation}
    p_{i} = \frac{k_i}{N}.
\end{equation}

\begin{equation}
    p_{i} \cdot \log_{2}p_{i} = \frac{k_i}{N} \cdot \log_{2}\frac{k_i}{N}.
\end{equation}

\begin{equation}
    p_{i} \cdot \log_{2}p_{i} = \frac{k_i}{N} \cdot (\log_{2}k_i - \log_{2}N).
\end{equation}

\begin{equation}
    H(X) = -(\frac{k_1}{N} \cdot (\log_{2}k_1 - \log_{2}N) + ... + \frac{k_{255}}{N} \cdot (\log_{2}k_{255} - \log_{2}N)).
\end{equation}

\begin{equation}
    H(X) = \frac{k_1}{N} \cdot ( \log_{2}N - \log_{2}k_1) + ... + \frac{k_{255}}{N} \cdot (\log_{2}N - \log_{2}k_{255}).
\end{equation}

\begin{equation}
    H(X) \cdot N = k_1 \cdot ( \log_{2}N - \log_{2}k_1) + ... + k_{255} \cdot (\log_{2}N - \log_{2}k_{255}).
\end{equation}

\begin{equation}
    N = PAGE\_SIZE.
\end{equation}

\section*{Биномиальный метод}

\begin{equation}
    H(X) = -\sum_{k = 0}^n (C_{n}^k \cdot P_{k} \cdot \log_{2}P_{k}).
\end{equation}

\begin{equation}\label{pk}
	P_{k} = p^k \cdot (1 - p)^{(n - k)}.
\end{equation} 

\begin{equation}
    p = \frac{x_i}{N \cdot 8}, x_i\text{ --- число единиц.}
\end{equation}

\begin{equation}\label{pk}
	P_{k} = (\frac{x_i}{(8N)})^k \cdot (1 - \frac{x_i}{(8N)})^{(n - k)}.
\end{equation}

\begin{equation}\label{pk}
	P_{k} = \frac{x_i^k}{(8N)^k} \cdot \frac{(8N - x_i)^{(n - k)}}{(8N)^{(n - k)}}.
\end{equation} 

\begin{equation}\label{pk}
	P_{k} = \frac{x_i^k \cdot (8N - x_i)^{(n - k)}}{(8N)^n}.
\end{equation}

\begin{equation}
    P_{k} \cdot \log_{2}P_{k} = \frac{x_i^k \cdot (8N - x_i)^{(n - k)}}{(8N)^n} \cdot (\log_{2}x_i^k \cdot (8N - x_i)^{(n - k)} - \log_{2}(8N)^n).
\end{equation}

\begin{equation}
    H(X) = -(C_{n}^0 \cdot \frac{x_i^0 \cdot (8N - x_i)^{(n - 0)}}{(8N)^n} \cdot (\log_{2}x_i^0 \cdot (8N - x_i)^{(n - 0)} - \log_{2}(8N)^n) + ...).
\end{equation}

\begin{equation}
    H(X) = (C_{n}^0 \cdot \frac{x_i^0 \cdot (8N - x_i)^{(n - 0)}}{(8N)^n} \cdot (\log_{2}(8N)^n - \log_{2}x_i^0 \cdot (8N - x_i)^{(n - 0)}) + ...).
\end{equation}

\begin{equation}
    H(X) \cdot (8N)^n = (C_{n}^0 \cdot x_i^0 \cdot (8N - x_i)^{(n - 0)} \cdot (\log_{2}(8N)^n - \log_{2}x_i^0 \cdot (8N - x_i)^{(n - 0)}) + ...).
\end{equation}

\begin{equation}
    n = 8, N = PAGE\_SIZE.
\end{equation}

\begin{equation}
    C_{8}^0 = 1, C_{8}^1 = 8, C_{8}^2 = 28, C_{8}^3 = 56, C_{8}^4 = 70, C_{8}^5 = 56, C_{8}^6 = 28, C_{8}^7 = 8, C_{8}^8 = 1.
\end{equation}

\end{document}